tests/coq/misc/Loops.v
@@ -22,8 +22,8 @@ Definition sum_fwd (n : nat) (max : u32) : result u32 :=
   sum_loop_fwd n max (0%u32) (0%u32)
 .
 
-(** [loops::sum_with_borrows] *)
-Fixpoint sum_with_borrows_loop_fwd
+(** [loops::sum_with_mut_borrows] *)
+Fixpoint sum_with_mut_borrows_loop_fwd
   (n : nat) (max : u32) (mi : u32) (ms : u32) : result u32 :=
   match n with
   | O => Fail_ OutOfFuel
@@ -32,14 +32,34 @@ Fixpoint sum_with_borrows_loop_fwd
     then (
       ms0 <- u32_add ms mi;
       mi0 <- u32_add mi 1%u32;
-      sum_with_borrows_loop_fwd n0 max mi0 ms0)
+      sum_with_mut_borrows_loop_fwd n0 max mi0 ms0)
     else u32_mul ms 2%u32
   end
 .
 
-(** [loops::sum_with_borrows] *)
-Definition sum_with_borrows_fwd (n : nat) (max : u32) : result u32 :=
-  sum_with_borrows_loop_fwd n max (0%u32) (0%u32)
+(** [loops::sum_with_mut_borrows] *)
+Definition sum_with_mut_borrows_fwd (n : nat) (max : u32) : result u32 :=
+  sum_with_mut_borrows_loop_fwd n max (0%u32) (0%u32)
+.
+
+(** [loops::sum_with_shared_borrows] *)
+Fixpoint sum_with_shared_borrows_loop_fwd
+  (n : nat) (max : u32) (i : u32) (s : u32) : result u32 :=
+  match n with
+  | O => Fail_ OutOfFuel
+  | S n0 =>
+    if i s< max
+    then (
+      i0 <- u32_add i 1%u32;
+      s0 <- u32_add s i0;
+      sum_with_shared_borrows_loop_fwd n0 max i0 s0)
+    else u32_mul s 2%u32
+  end
+.
+
+(** [loops::sum_with_shared_borrows] *)
+Definition sum_with_shared_borrows_fwd (n : nat) (max : u32) : result u32 :=
+  sum_with_shared_borrows_loop_fwd n max (0%u32) (0%u32)
 .
 
 (** [loops::List] *)
@@ -100,6 +120,28 @@ Definition list_nth_mut_loop_back
   result (List_t T)
   :=
   list_nth_mut_loop_loop_back T n ls i ret
+.
+
+(** [loops::list_nth_shared_loop] *)
+Fixpoint list_nth_shared_loop_loop_fwd
+  (T : Type) (n : nat) (ls : List_t T) (i : u32) : result T :=
+  match n with
+  | O => Fail_ OutOfFuel
+  | S n0 =>
+    match ls with
+    | ListCons x tl =>
+      if i s= 0%u32
+      then Return x
+      else (i0 <- u32_sub i 1%u32; list_nth_shared_loop_loop_fwd T n0 tl i0)
+    | ListNil => Fail_ Failure
+    end
+  end
+.
+
+(** [loops::list_nth_shared_loop] *)
+Definition list_nth_shared_loop_fwd
+  (T : Type) (n : nat) (ls : List_t T) (i : u32) : result T :=
+  list_nth_shared_loop_loop_fwd T n ls i
 .
 
 (** [loops::list_nth_mut_loop_pair] *)
@@ -200,6 +242,38 @@ Definition list_nth_mut_loop_pair_back'b
   list_nth_mut_loop_pair_loop_back'b T n ls0 ls1 i ret
 .
 
+(** [loops::list_nth_shared_loop_pair] *)
+Fixpoint list_nth_shared_loop_pair_loop_fwd
+  (T : Type) (n : nat) (l : List_t T) (l0 : List_t T) (i : u32) :
+  result (T * T)
+  :=
+  match n with
+  | O => Fail_ OutOfFuel
+  | S n0 =>
+    match l with
+    | ListCons x0 tl0 =>
+      match l0 with
+      | ListCons x1 tl1 =>
+        if i s= 0%u32
+        then Return (x0, x1)
+        else (
+          i0 <- u32_sub i 1%u32;
+          list_nth_shared_loop_pair_loop_fwd T n0 tl0 tl1 i0)
+      | ListNil => Fail_ Failure
+      end
+    | ListNil => Fail_ Failure
+    end
+  end
+.
+
+(** [loops::list_nth_shared_loop_pair] *)
+Definition list_nth_shared_loop_pair_fwd
+  (T : Type) (n : nat) (ls0 : List_t T) (ls1 : List_t T) (i : u32) :
+  result (T * T)
+  :=
+  list_nth_shared_loop_pair_loop_fwd T n ls0 ls1 i
+.
+
 (** [loops::list_nth_mut_loop_pair_merge] *)
 Fixpoint list_nth_mut_loop_pair_merge_loop_fwd
   (T : Type) (n : nat) (l : List_t T) (l0 : List_t T) (i : u32) :
@@ -266,6 +340,300 @@ Definition list_nth_mut_loop_pair_merge_back
   result ((List_t T) * (List_t T))
   :=
   list_nth_mut_loop_pair_merge_loop_back T n ls0 ls1 i ret
+.
+
+(** [loops::list_nth_shared_loop_pair_merge] *)
+Fixpoint list_nth_shared_loop_pair_merge_loop_fwd
+  (T : Type) (n : nat) (l : List_t T) (l0 : List_t T) (i : u32) :
+  result (T * T)
+  :=
+  match n with
+  | O => Fail_ OutOfFuel
+  | S n0 =>
+    match l with
+    | ListCons x0 tl0 =>
+      match l0 with
+      | ListCons x1 tl1 =>
+        if i s= 0%u32
+        then Return (x0, x1)
+        else (
+          i0 <- u32_sub i 1%u32;
+          list_nth_shared_loop_pair_merge_loop_fwd T n0 tl0 tl1 i0)
+      | ListNil => Fail_ Failure
+      end
+    | ListNil => Fail_ Failure
+    end
+  end
+.
+
+(** [loops::list_nth_shared_loop_pair_merge] *)
+Definition list_nth_shared_loop_pair_merge_fwd
+  (T : Type) (n : nat) (ls0 : List_t T) (ls1 : List_t T) (i : u32) :
+  result (T * T)
+  :=
+  list_nth_shared_loop_pair_merge_loop_fwd T n ls0 ls1 i
+.
+
+(** [loops::list_nth_mut_shared_loop_pair] *)
+Fixpoint list_nth_mut_shared_loop_pair_loop_fwd
+  (T : Type) (n : nat) (l : List_t T) (l0 : List_t T) (i : u32) :
+  result (T * T)
+  :=
+  match n with
+  | O => Fail_ OutOfFuel
+  | S n0 =>
+    match l with
+    | ListCons x0 tl0 =>
+      match l0 with
+      | ListCons x1 tl1 =>
+        if i s= 0%u32
+        then Return (x0, x1)
+        else (
+          i0 <- u32_sub i 1%u32;
+          list_nth_mut_shared_loop_pair_loop_fwd T n0 tl0 tl1 i0)
+      | ListNil => Fail_ Failure
+      end
+    | ListNil => Fail_ Failure
+    end
+  end
+.
+
+(** [loops::list_nth_mut_shared_loop_pair] *)
+Definition list_nth_mut_shared_loop_pair_fwd
+  (T : Type) (n : nat) (ls0 : List_t T) (ls1 : List_t T) (i : u32) :
+  result (T * T)
+  :=
+  list_nth_mut_shared_loop_pair_loop_fwd T n ls0 ls1 i
+.
+
+(** [loops::list_nth_mut_shared_loop_pair] *)
+Fixpoint list_nth_mut_shared_loop_pair_loop_back
+  (T : Type) (n : nat) (l : List_t T) (l0 : List_t T) (i : u32) (ret : T) :
+  result (List_t T)
+  :=
+  match n with
+  | O => Fail_ OutOfFuel
+  | S n0 =>
+    match l with
+    | ListCons x0 tl0 =>
+      match l0 with
+      | ListCons x1 tl1 =>
+        if i s= 0%u32
+        then Return (ListCons ret tl0)
+        else (
+          i0 <- u32_sub i 1%u32;
+          l1 <- list_nth_mut_shared_loop_pair_loop_back T n0 tl0 tl1 i0 ret;
+          Return (ListCons x0 l1))
+      | ListNil => Fail_ Failure
+      end
+    | ListNil => Fail_ Failure
+    end
+  end
+.
+
+(** [loops::list_nth_mut_shared_loop_pair] *)
+Definition list_nth_mut_shared_loop_pair_back
+  (T : Type) (n : nat) (ls0 : List_t T) (ls1 : List_t T) (i : u32) (ret : T) :
+  result (List_t T)
+  :=
+  list_nth_mut_shared_loop_pair_loop_back T n ls0 ls1 i ret
+.
+
+(** [loops::list_nth_mut_shared_loop_pair_merge] *)
+Fixpoint list_nth_mut_shared_loop_pair_merge_loop_fwd
+  (T : Type) (n : nat) (l : List_t T) (l0 : List_t T) (i : u32) :
+  result (T * T)
+  :=
+  match n with
+  | O => Fail_ OutOfFuel
+  | S n0 =>
+    match l with
+    | ListCons x0 tl0 =>
+      match l0 with
+      | ListCons x1 tl1 =>
+        if i s= 0%u32
+        then Return (x0, x1)
+        else (
+          i0 <- u32_sub i 1%u32;
+          list_nth_mut_shared_loop_pair_merge_loop_fwd T n0 tl0 tl1 i0)
+      | ListNil => Fail_ Failure
+      end
+    | ListNil => Fail_ Failure
+    end
+  end
+.
+
+(** [loops::list_nth_mut_shared_loop_pair_merge] *)
+Definition list_nth_mut_shared_loop_pair_merge_fwd
+  (T : Type) (n : nat) (ls0 : List_t T) (ls1 : List_t T) (i : u32) :
+  result (T * T)
+  :=
+  list_nth_mut_shared_loop_pair_merge_loop_fwd T n ls0 ls1 i
+.
+
+(** [loops::list_nth_mut_shared_loop_pair_merge] *)
+Fixpoint list_nth_mut_shared_loop_pair_merge_loop_back
+  (T : Type) (n : nat) (l : List_t T) (l0 : List_t T) (i : u32) (ret : T) :
+  result (List_t T)
+  :=
+  match n with
+  | O => Fail_ OutOfFuel
+  | S n0 =>
+    match l with
+    | ListCons x0 tl0 =>
+      match l0 with
+      | ListCons x1 tl1 =>
+        if i s= 0%u32
+        then Return (ListCons ret tl0)
+        else (
+          i0 <- u32_sub i 1%u32;
+          l1 <-
+            list_nth_mut_shared_loop_pair_merge_loop_back T n0 tl0 tl1 i0 ret;
+          Return (ListCons x0 l1))
+      | ListNil => Fail_ Failure
+      end
+    | ListNil => Fail_ Failure
+    end
+  end
+.
+
+(** [loops::list_nth_mut_shared_loop_pair_merge] *)
+Definition list_nth_mut_shared_loop_pair_merge_back
+  (T : Type) (n : nat) (ls0 : List_t T) (ls1 : List_t T) (i : u32) (ret : T) :
+  result (List_t T)
+  :=
+  list_nth_mut_shared_loop_pair_merge_loop_back T n ls0 ls1 i ret
+.
+
+(** [loops::list_nth_shared_mut_loop_pair] *)
+Fixpoint list_nth_shared_mut_loop_pair_loop_fwd
+  (T : Type) (n : nat) (l : List_t T) (l0 : List_t T) (i : u32) :
+  result (T * T)
+  :=
+  match n with
+  | O => Fail_ OutOfFuel
+  | S n0 =>
+    match l with
+    | ListCons x0 tl0 =>
+      match l0 with
+      | ListCons x1 tl1 =>
+        if i s= 0%u32
+        then Return (x0, x1)
+        else (
+          i0 <- u32_sub i 1%u32;
+          list_nth_shared_mut_loop_pair_loop_fwd T n0 tl0 tl1 i0)
+      | ListNil => Fail_ Failure
+      end
+    | ListNil => Fail_ Failure
+    end
+  end
+.
+
+(** [loops::list_nth_shared_mut_loop_pair] *)
+Definition list_nth_shared_mut_loop_pair_fwd
+  (T : Type) (n : nat) (ls0 : List_t T) (ls1 : List_t T) (i : u32) :
+  result (T * T)
+  :=
+  list_nth_shared_mut_loop_pair_loop_fwd T n ls0 ls1 i
+.
+
+(** [loops::list_nth_shared_mut_loop_pair] *)
+Fixpoint list_nth_shared_mut_loop_pair_loop_back
+  (T : Type) (n : nat) (l : List_t T) (l0 : List_t T) (i : u32) (ret : T) :
+  result (List_t T)
+  :=
+  match n with
+  | O => Fail_ OutOfFuel
+  | S n0 =>
+    match l with
+    | ListCons x0 tl0 =>
+      match l0 with
+      | ListCons x1 tl1 =>
+        if i s= 0%u32
+        then Return (ListCons ret tl1)
+        else (
+          i0 <- u32_sub i 1%u32;
+          l1 <- list_nth_shared_mut_loop_pair_loop_back T n0 tl0 tl1 i0 ret;
+          Return (ListCons x1 l1))
+      | ListNil => Fail_ Failure
+      end
+    | ListNil => Fail_ Failure
+    end
+  end
+.
+
+(** [loops::list_nth_shared_mut_loop_pair] *)
+Definition list_nth_shared_mut_loop_pair_back
+  (T : Type) (n : nat) (ls0 : List_t T) (ls1 : List_t T) (i : u32) (ret : T) :
+  result (List_t T)
+  :=
+  list_nth_shared_mut_loop_pair_loop_back T n ls0 ls1 i ret
+.
+
+(** [loops::list_nth_shared_mut_loop_pair_merge] *)
+Fixpoint list_nth_shared_mut_loop_pair_merge_loop_fwd
+  (T : Type) (n : nat) (l : List_t T) (l0 : List_t T) (i : u32) :
+  result (T * T)
+  :=
+  match n with
+  | O => Fail_ OutOfFuel
+  | S n0 =>
+    match l with
+    | ListCons x0 tl0 =>
+      match l0 with
+      | ListCons x1 tl1 =>
+        if i s= 0%u32
+        then Return (x0, x1)
+        else (
+          i0 <- u32_sub i 1%u32;
+          list_nth_shared_mut_loop_pair_merge_loop_fwd T n0 tl0 tl1 i0)
+      | ListNil => Fail_ Failure
+      end
+    | ListNil => Fail_ Failure
+    end
+  end
+.
+
+(** [loops::list_nth_shared_mut_loop_pair_merge] *)
+Definition list_nth_shared_mut_loop_pair_merge_fwd
+  (T : Type) (n : nat) (ls0 : List_t T) (ls1 : List_t T) (i : u32) :
+  result (T * T)
+  :=
+  list_nth_shared_mut_loop_pair_merge_loop_fwd T n ls0 ls1 i
+.
+
+(** [loops::list_nth_shared_mut_loop_pair_merge] *)
+Fixpoint list_nth_shared_mut_loop_pair_merge_loop_back
+  (T : Type) (n : nat) (l : List_t T) (l0 : List_t T) (i : u32) (ret : T) :
+  result (List_t T)
+  :=
+  match n with
+  | O => Fail_ OutOfFuel
+  | S n0 =>
+    match l with
+    | ListCons x0 tl0 =>
+      match l0 with
+      | ListCons x1 tl1 =>
+        if i s= 0%u32
+        then Return (ListCons ret tl1)
+        else (
+          i0 <- u32_sub i 1%u32;
+          l1 <-
+            list_nth_shared_mut_loop_pair_merge_loop_back T n0 tl0 tl1 i0 ret;
+          Return (ListCons x1 l1))
+      | ListNil => Fail_ Failure
+      end
+    | ListNil => Fail_ Failure
+    end
+  end
+.
+
+(** [loops::list_nth_shared_mut_loop_pair_merge] *)
+Definition list_nth_shared_mut_loop_pair_merge_back
+  (T : Type) (n : nat) (ls0 : List_t T) (ls1 : List_t T) (i : u32) (ret : T) :
+  result (List_t T)
+  :=
+  list_nth_shared_mut_loop_pair_merge_loop_back T n ls0 ls1 i ret
 .
 
 End Loops .
